tie some global things together

theories/sim/instance.v
@@ -5,26 +5,27 @@ Notation "r ⊨{ n , fs , ft } ( es , σs ) ≥ ( et , σt ) : Φ" :=
   (sim_local_body wsat vrel fs ft r n%nat es%E σs et%E σt Φ)
   (at level 70, format "'[hv' r  '/' ⊨{ n , fs , ft }  '/  ' '[ ' ( es ,  '/' σs ) ']'  '/' ≥  '/  ' '[ ' ( et ,  '/' σt ) ']'  '/' :  Φ ']'").
 
-Notation "⊨ᶠ{ fs , ft } f1 ≥ f2" :=
-  (sim_local_fun wsat vrel fs ft end_call_sat f1 f2)
-  (at level 70, f1, f2 at next level, format "⊨ᶠ{ fs , ft }  f1  ≥  f2").
 
-Lemma sim_body_result fs ft r n es et σs σt Φ :
-  (✓ r → Φ r n es σs et σt : Prop) →
-  r ⊨{S n,fs,ft} (of_result es, σs) ≥ (of_result et, σt) : Φ.
-Proof.
-  intros POST. pfold.  split; last first.
-  { constructor 1. intros vt' ? STEPT'. exfalso.
-    apply result_tstep_stuck in STEPT'. by rewrite to_of_result in STEPT'. }
-  { move => ? /= Eqvt'. symmetry in Eqvt'. simplify_eq.
-    exists es, σs, r, n. split; last split.
-    - right. split; [lia|]. eauto.
-    - eauto.
-    - rewrite to_of_result in Eqvt'. simplify_eq.
-      apply POST. by destruct WSAT as (?&?&?%cmra_valid_op_r &?). }
-  { left. rewrite to_of_result. by eexists. }
-Qed.
+(** "modular" simulation relations dont make assumptions
+about the global fn table.
+This is very weak! A stronger version would, instead of universally quantifying the
+fn table, allow giving a lower bound. But this is good enough for now.
 
+This could be done in general, but we just do it for the instance. *)
+Definition sim_mod_fun f1 f2 :=
+  ∀ fs ft, sim_local_funs_lookup fs ft → sim_local_fun wsat vrel fs ft end_call_sat f1 f2.
+
+Definition sim_mod_funs (fns fnt: fn_env) :=
+  ∀ name fn_src, fns !! name = Some fn_src → ∃ fn_tgt,
+    fnt !! name = Some fn_tgt ∧
+    length fn_src.(fun_b) = length fn_tgt.(fun_b) ∧
+    sim_mod_fun fn_src fn_tgt.
+
+Notation "⊨ᶠ f1 ≥ f2" :=
+  (sim_mod_fun f1 f2)
+  (at level 70, f1, f2 at next level, format "⊨ᶠ  f1  ≥  f2").
+
+(** The modular version permits insertion. *)
 Lemma sim_local_funs_lookup_insert fns fnt x fs ft :
   length fns.(fun_b) = length fnt.(fun_b) →
   sim_local_funs_lookup fs ft →
@@ -39,58 +40,35 @@ Proof.
     rewrite lookup_insert_ne //.
 Qed.
 
-Lemma sim_local_body_insert fs ft fns fnt x r n es et σs σt Φ 
-  (FRESH : fs !! x = None)
-  (HOLD: sim_local_funs_lookup fs ft) :
-  ⊨ᶠ{fs,ft} fns ≥ fnt →
-  r ⊨{n,fs,ft} (es, σs) ≥ (et, σt) : Φ →
-  r ⊨{n,<[x:=fns]> fs,<[x:=fnt]> ft} (es, σs) ≥ (et, σt) : Φ.
-Proof.
-  intros FUN. revert r n es et σs σt Φ. pcofix CIH.
-  intros r1 n es et σs σt Φ SIM. punfold SIM. pfold.
-  intros NT r_f WSAT.
-  have NT2: never_stuck fs es σs. { admit. }
-  specialize (SIM NT2 r_f WSAT) as [NS TE ST]. split.
-  - destruct NS as [|RED]; [by left|]. right. admit.
-  - intros vt Eqvt.
-    specialize (TE _ Eqvt) as (vs' & σs' & r' & n' & STEPS' & WSAT' & HΦ).
-    exists vs', σs', r', n'. split; last split; [|done..].
-    { destruct STEPS' as [STEPS'|]; [|by right]. left. admit. }
-  - inversion ST.
-    + constructor 1.
-      intros et' σt' STEPT.
-      have STEPT2: (et, σt) ~{ft}~> (et', σt'). { admit. }
-      specialize (STEP _ _ STEPT2) as (vs' & σs' & r' & n' & STEPS' & WSAT' & CONT).
-      exists vs', σs', r', n'. split; last split; [|done|].
-      { admit. }
-      pclearbot. right. by apply CIH.
-    + econstructor 2; eauto.
-      { instantiate (1:= Ks). admit. }
-      intros r' vs vt σs' σt' VREL' WSAT' STACK'.
-      specialize (CONT r' vs vt σs' σt' VREL' WSAT' STACK') as [n' CONT].
-      exists n'. pclearbot. right. by apply CIH.
-Admitted.
-
-Lemma sim_local_funs_insert fns fnt x fs ft :
+Lemma sim_mod_funs_insert fs ft x fns fnt :
   length fns.(fun_b) = length fnt.(fun_b) →
-  fs !! x = None →
-  (* FIXME: add notation for this. Probably replacing ⊨ᶠ. *)
-  (∀ fs ft, sim_local_funs_lookup fs ft → ⊨ᶠ{ fs , ft } fns ≥ fnt) →
-  sim_local_funs wsat vrel fs ft end_call_sat →
-  sim_local_funs wsat vrel (<[x:=fns]>fs) (<[x:=fnt]>ft) end_call_sat.
+  (⊨ᶠ fns ≥ fnt) →
+  sim_mod_funs fs ft →
+  sim_mod_funs (<[x:=fns]>fs) (<[x:=fnt]>ft).
 Proof.
-  intros ?? Hnew Hold. intros f fn_src.
+  intros ? Hnew Hold. intros f fn_src.
   destruct (decide (x=f)) as [->|Hne].
   - rewrite lookup_insert=>[=?]. subst. exists fnt. rewrite lookup_insert.
     split; first done. split; first done. apply Hnew.
-    apply sim_local_funs_lookup_insert; first done.
-    exact: sim_local_funs_to_lookup.
   - rewrite lookup_insert_ne // =>Hlk.
     destruct (Hold _ _ Hlk) as (f_tgt & ? & ? & Hf). exists f_tgt.
-    rewrite lookup_insert_ne //. split; first done.
-    split; first done.
-    have ? : sim_local_funs_lookup fs ft by eapply sim_local_funs_to_lookup.
-    intros r es et vs vt σs σt VREL SUBS SUBT.
-    specialize (Hf r es et vs vt σs σt VREL SUBS SUBT) as [n Hf].
-    exists n. apply sim_local_body_insert; [done..|by apply Hnew|done].
+    rewrite lookup_insert_ne //.
+Qed.
+
+Lemma sim_mod_funs_to_lookup fs ft:
+  sim_mod_funs fs ft → sim_local_funs_lookup fs ft.
+Proof.
+  intros Hlf name fns Hlk. destruct (Hlf _ _ Hlk) as (fnt & ? & ? & ?).
+  eauto.
+Qed.
+
+(** Once we got all things together, we can get the whole-program
+assumption. *)
+Lemma sim_mod_funs_local fs ft :
+  sim_mod_funs fs ft →
+  sim_local_funs wsat vrel fs ft end_call_sat.
+Proof.
+  intros Hmod. intros f fn_src Hlk.
+  destruct (Hmod _ _ Hlk) as (fn_tgt & ? & ? & ?). exists fn_tgt.
+  eauto using sim_mod_funs_to_lookup.
 Qed.
