theories/sim/refl.v
@@ -1,0 +1,9 @@
+From stbor.lang Require Import lang.
+From stbor.sim Require Import refl_step.
+
+Set Default Proof Using "Type".
+
+Lemma sim_mod_funs_refl prog :
+  sim_mod_funs prog prog.
+Proof.
+Admitted.
