theories/sim/refl_step.v
@@ -1,7 +1,7 @@
 From iris.algebra Require Import local_updates.
 
 From stbor.lang Require Import steps_progress steps_inversion steps_retag.
-From stbor.sim Require Export instance.
+From stbor.sim Require Export instance body.
 
 Set Default Proof Using "Type".
 
